SStructTT/MartinLof/Normalization.lean
@@ -4,4 +4,4 @@ open ARS
 namespace MartinLof
 
 -- Postulate: Martin-Lof Type Theory is strongly normalizing.
-axiom Typed.sn {Γ m A} : Γ ⊢ m : A -> SN Step m
+axiom Typed.normalization {Γ m A} : Γ ⊢ m : A -> SN Step m
